src/core/DY.Core.Trace.SplitUtils.Derived.fst
@@ -28,6 +28,23 @@ let trace_split_at (#a:Type) (tr:trace_ a) (e:trace_entry_ a{entry_exists tr e})
 
 /// Derived functions for trace arithmetic
 
+let trace_subtract_nil (#label_t:Type) (tr:trace_ label_t)
+  : Lemma
+    ((tr <--> Nil) == tr)
+    [SMTPat (tr <--> Nil)]
+  = trace_concat_subtract Nil tr
+
+let trace_subtract_itself (#label_t:Type) (tr:trace_ label_t)
+  : Lemma
+    ((tr <--> tr) == Nil)
+    [SMTPat (tr <--> tr)]
+  = trace_concat_subtract tr Nil
+
+let trace_concat_snoc_right (#label_t:Type) (tr1 tr2:trace_ label_t) (e:trace_entry_ label_t)
+  : Lemma
+    (tr1 <++> (Snoc tr2 e) == Snoc (tr1 <++> tr2) e)
+  = trace_concat_assoc tr1 tr2 (Snoc Nil e)
+
 let trace_subtract_concat_left (#label_t:Type) (tr1 tr2 tr3:trace_ label_t)
   : Lemma
     (requires tr1 <$ tr2)
